code/bignum/Hacl.Spec.Exponentiation.fst
@@ -1,0 +1,147 @@
+module Hacl.Spec.Exponentiation
+
+open FStar.Mul
+open Lib.IntTypes
+
+module LSeq = Lib.Sequence
+module BSeq = Lib.ByteSequence
+module Loops = Lib.LoopCombinators
+
+module S = Lib.Exponentiation
+module SB = Hacl.Spec.Bignum.Base
+
+#reset-options "--z3rlimit 50 --fuel 0 --ifuel 0"
+
+
+val precomp_table_inv_lemma_j:
+    #a_t:inttype_a
+  -> len:size_nat{len > 0}
+  -> ctx_len:size_nat
+  -> k:to_comm_monoid a_t len ctx_len
+  -> a:LSeq.lseq (uint_t a_t SEC) len
+  -> table_len:size_nat{table_len * len <= max_size_t}
+  -> table1:LSeq.lseq (uint_t a_t SEC) (table_len * len)
+  -> table2:LSeq.lseq (uint_t a_t SEC) (table_len * len)
+  -> i:nat{i <= table_len}
+  -> j:nat{j < i} -> Lemma
+  (requires
+    LSeq.sub table1 0 (i * len) == LSeq.sub table2 0 (i * len) /\
+    precomp_table_inv len ctx_len k a table_len table1 j)
+  (ensures
+    precomp_table_inv len ctx_len k a table_len table2 j)
+
+let precomp_table_inv_lemma_j #a_t len ctx_len k a table_len table1 table2 i j =
+  assert (precomp_table_inv len ctx_len k a table_len table1 j);
+  Math.Lemmas.lemma_mult_le_right len (j + 1) table_len;
+  let bj1 = LSeq.sub table1 (j * len) len in
+  let bj2 = LSeq.sub table2 (j * len) len in
+
+  let aux (l:nat{l < len}) : Lemma (LSeq.index bj1 l == LSeq.index bj2 l) =
+    Seq.lemma_index_slice table1 (j * len) (j * len + len) l;
+    //assert (LSeq.index bj1 l == LSeq.index table1 (j * len + l));
+    Seq.lemma_index_slice table2 (j * len) (j * len + len) l;
+    //assert (LSeq.index bj2 l == LSeq.index table2 (j * len + l));
+    Seq.lemma_index_slice table1 0 (i * len) (j * len + l);
+    Seq.lemma_index_slice table2 0 (i * len) (j * len + l);
+    //assert (LSeq.index table1 (j * len + l) == LSeq.index table2 (j * len + l));
+    assert (LSeq.index bj1 l == LSeq.index bj2 l) in
+
+  Classical.forall_intro aux;
+  LSeq.eq_intro bj1 bj2;
+  assert (precomp_table_inv len ctx_len k a table_len table2 j)
+
+
+let precomp_table_inv_lemma #a_t len ctx_len k a table_len table1 table2 i =
+  let aux (j:nat{j < i}) : Lemma (precomp_table_inv len ctx_len k a table_len table2 j) =
+    assert (precomp_table_inv len ctx_len k a table_len table1 j);
+    precomp_table_inv_lemma_j #a_t len ctx_len k a table_len table1 table2 i j;
+    assert (precomp_table_inv len ctx_len k a table_len table2 j) in
+
+  Classical.forall_intro aux
+
+
+
+val table_select_consttime_f:
+    #a_t:inttype_a
+  -> len:size_nat{len > 0}
+  -> table_len:size_nat{1 < table_len /\ table_len * len <= max_size_t}
+  -> table:LSeq.lseq (uint_t a_t SEC) (table_len * len)
+  -> i:uint_t a_t SEC{v i < table_len}
+  -> j:size_nat{j < table_len - 1}
+  -> acc:LSeq.lseq (uint_t a_t SEC) len ->
+  LSeq.lseq (uint_t a_t SEC) len
+
+let table_select_consttime_f #a_t len table_len table i j acc =
+  let c = eq_mask i (SB.size_to_limb (size j +! 1ul)) in
+  //assert (v c == (if v i = v j + 1 then ones_v a_t else 0));
+
+  Math.Lemmas.lemma_mult_le_right len (j + 2) table_len;
+  let res_j = LSeq.sub table ((j + 1) * len) len in
+  let acc = LSeq.map2 (SB.mask_select c) res_j acc in
+  acc
+
+
+let table_select_consttime #a_t len table_len table i =
+  let res = LSeq.sub table 0 len in
+  Loops.repeati (table_len - 1) (table_select_consttime_f #a_t len table_len table i) res
+
+
+val table_select_consttime_f_lemma:
+    #a_t:inttype_a
+  -> len:size_nat{len > 0}
+  -> table_len:size_nat{1 < table_len /\ table_len * len <= max_size_t}
+  -> table:LSeq.lseq (uint_t a_t SEC) (table_len * len)
+  -> i:uint_t a_t SEC{v i < table_len}
+  -> j:size_nat{j < table_len - 1}
+  -> acc:LSeq.lseq (uint_t a_t SEC) len ->
+  Lemma (
+    let res = table_select_consttime_f len table_len table i j acc in
+    Math.Lemmas.lemma_mult_le_right len (j + 2) table_len;
+    let res_j = LSeq.sub table ((j + 1) * len) len in
+    res == (if v i = j + 1 then res_j else acc))
+
+let table_select_consttime_f_lemma #a_t len table_len table i j acc =
+  let c = eq_mask i (SB.size_to_limb (size (j + 1))) in
+  assert (v c == (if v i = j + 1 then ones_v a_t else 0));
+
+  Math.Lemmas.lemma_mult_le_right len (j + 2) table_len;
+  let res_j = LSeq.sub table ((j + 1) * len) len in
+  let res = LSeq.map2 (SB.mask_select c) res_j acc in
+  SB.lseq_mask_select_lemma res_j acc c
+
+
+val table_select_consttime_loop_lemma:
+    #a_t:inttype_a
+  -> len:size_nat{len > 0}
+  -> table_len:size_nat{1 < table_len /\ table_len * len <= max_size_t}
+  -> table:LSeq.lseq (uint_t a_t SEC) (table_len * len)
+  -> i:uint_t a_t SEC{v i < table_len} ->
+  Pure (LSeq.lseq (uint_t a_t SEC) len)
+  (requires True)
+  (ensures  fun res ->
+    let res0 = LSeq.sub table 0 len in
+    Math.Lemmas.lemma_mult_le_right len (v i + 1) table_len;
+    res == Loops.repeati (table_len - 1) (table_select_consttime_f len table_len table i) res0 /\
+    res == LSeq.sub table (v i * len) len)
+
+let table_select_consttime_loop_lemma #a_t len table_len table i =
+  let f = table_select_consttime_f len table_len table i in
+  let res0 = LSeq.sub table 0 len in
+  Math.Lemmas.lemma_mult_le_right len (v i + 1) table_len;
+
+  Loops.eq_repeati0 (table_len - 1) f res0;
+  Loops.repeati_inductive (table_len - 1)
+  (fun j priv ->
+    priv == Loops.repeati j f res0 /\
+    priv == (if j >= v i then LSeq.sub table (v i * len) len else res0))
+  (fun j priv ->
+    Loops.unfold_repeati (j + 1) f res0 j;
+    let res = f j priv in
+    table_select_consttime_f_lemma len table_len table i j priv;
+    Math.Lemmas.lemma_mult_le_right len (j + 2) table_len;
+    let res_j = LSeq.sub table ((j + 1) * len) len in
+    assert (res == (if v i = j + 1 then res_j else priv));
+    res) res0
+
+let table_select_consttime_lemma #a_t len table_len table i =
+  let _ = table_select_consttime_loop_lemma len table_len table i in ()
