code/bignum/Hacl.Spec.Exponentiation.fsti
@@ -1,0 +1,77 @@
+module Hacl.Spec.Exponentiation
+
+open FStar.Mul
+open Lib.IntTypes
+
+module LSeq = Lib.Sequence
+module BSeq = Lib.ByteSequence
+module Loops = Lib.LoopCombinators
+
+module S = Lib.Exponentiation
+
+#reset-options "--z3rlimit 50 --fuel 0 --ifuel 0"
+
+inline_for_extraction noextract
+let inttype_a = t:inttype{t = U32 \/ t = U64}
+
+inline_for_extraction noextract
+class to_comm_monoid (a_t:inttype_a) (len:size_nat{len > 0}) (ctx_len:size_nat) = {
+  a_spec: Type0;
+  comm_monoid: S.comm_monoid a_spec;
+  linv_ctx: LSeq.lseq (uint_t a_t SEC) ctx_len -> Type0;
+  linv: LSeq.lseq (uint_t a_t SEC) len -> Type0;
+  refl: x:LSeq.lseq (uint_t a_t SEC) len{linv x} -> GTot a_spec;
+}
+
+
+inline_for_extraction noextract
+let precomp_table_inv
+  (#a_t:inttype_a)
+  (len:size_nat{len > 0})
+  (ctx_len:size_nat)
+  (k:to_comm_monoid a_t len ctx_len)
+  (a:LSeq.lseq (uint_t a_t SEC) len)
+  (table_len:size_nat{table_len * len <= max_size_t})
+  (table:LSeq.lseq (uint_t a_t SEC) (table_len * len))
+  (j:nat{j < table_len}) : Type0
+ =
+  Math.Lemmas.lemma_mult_le_right len (j + 1) table_len;
+  let bj = LSeq.sub table (j * len) len in
+  k.linv bj /\ k.linv a /\
+  k.refl bj == S.pow k.comm_monoid (k.refl a) j
+
+
+val precomp_table_inv_lemma:
+    #a_t:inttype_a
+  -> len:size_nat{len > 0}
+  -> ctx_len:size_nat
+  -> k:to_comm_monoid a_t len ctx_len
+  -> a:LSeq.lseq (uint_t a_t SEC) len
+  -> table_len:size_nat{table_len * len <= max_size_t}
+  -> table1:LSeq.lseq (uint_t a_t SEC) (table_len * len)
+  -> table2:LSeq.lseq (uint_t a_t SEC) (table_len * len)
+  -> i:nat{i <= table_len} -> Lemma
+  (requires
+    LSeq.sub table1 0 (i * len) == LSeq.sub table2 0 (i * len) /\
+    (forall (j:nat{j < i}). precomp_table_inv len ctx_len k a table_len table1 j))
+  (ensures
+    (forall (j:nat{j < i}). precomp_table_inv len ctx_len k a table_len table2 j))
+
+//`consttime` doesn't mean anything at the spec level
+val table_select_consttime:
+    #a_t:inttype_a
+  -> len:size_nat{len > 0}
+  -> table_len:size_nat{1 < table_len /\ table_len * len <= max_size_t}
+  -> table:LSeq.lseq (uint_t a_t SEC) (table_len * len)
+  -> i:uint_t a_t SEC{v i < table_len} ->
+  LSeq.lseq (uint_t a_t SEC) len
+
+
+val table_select_consttime_lemma:
+    #a_t:inttype_a
+  -> len:size_nat{len > 0}
+  -> table_len:size_nat{1 < table_len /\ table_len * len <= max_size_t}
+  -> table:LSeq.lseq (uint_t a_t SEC) (table_len * len)
+  -> i:uint_t a_t SEC{v i < table_len} ->
+  Lemma (Math.Lemmas.lemma_mult_le_right len (v i + 1) table_len;
+    table_select_consttime len table_len table i == LSeq.sub table (v i * len) len)
